access: Interrupt_AC arch split
Signed-off-by: Ryan Barry <ryan.barry@unsw.edu.au>

proof/access-control/Interrupt_AC.thy
@@ -6,58 +6,11 @@
 
 theory Interrupt_AC
 imports
-  Finalise_AC
+  ArchFinalise_AC
 begin
 
-context begin interpretation Arch . (*FIXME: arch_split*)
 
-definition
-  arch_authorised_irq_ctl_inv :: "'a PAS \<Rightarrow> Invocations_A.arch_irq_control_invocation \<Rightarrow> bool"
-where
-  "arch_authorised_irq_ctl_inv aag cinv \<equiv>
-     case cinv of
-         (ArchIRQControlIssue irq x1 x2 trigger) \<Rightarrow>
-                                 is_subject aag (fst x1) \<and> is_subject aag (fst x2) \<and>
-                                 (pasSubject aag, Control, pasIRQAbs aag irq) \<in> pasPolicy aag"
-
-definition
-  authorised_irq_ctl_inv :: "'a PAS \<Rightarrow> Invocations_A.irq_control_invocation \<Rightarrow> bool"
-where
-  "authorised_irq_ctl_inv aag cinv \<equiv>
-     case cinv of
-         IRQControl irq x1 x2 \<Rightarrow> is_subject aag (fst x1) \<and> is_subject aag (fst x2) \<and>
-                                  (pasSubject aag, Control, pasIRQAbs aag irq) \<in> pasPolicy aag
-        | ArchIRQControl acinv \<Rightarrow> arch_authorised_irq_ctl_inv aag acinv"
-
-lemma arch_invoke_irq_control_pas_refined:
-  "\<lbrace>pas_refined aag and valid_mdb and arch_irq_control_inv_valid irq_ctl_inv and
-     K (arch_authorised_irq_ctl_inv aag irq_ctl_inv)\<rbrace>
-     arch_invoke_irq_control irq_ctl_inv
-   \<lbrace>\<lambda>rv. pas_refined aag\<rbrace>"
-  apply (cases irq_ctl_inv; simp)
-  apply (wpsimp wp: cap_insert_pas_refined_not_transferable)
-  apply (clarsimp simp: cte_wp_at_caps_of_state clas_no_asid cap_links_irq_def
-                        arch_authorised_irq_ctl_inv_def aag_cap_auth_def
-                        arch_irq_control_inv_valid_def)
-  done
-
-lemma invoke_irq_control_pas_refined:
-  "\<lbrace>pas_refined aag and valid_mdb and irq_control_inv_valid irq_ctl_inv
-      and K (authorised_irq_ctl_inv aag irq_ctl_inv)\<rbrace>
-     invoke_irq_control irq_ctl_inv
-   \<lbrace>\<lambda>rv. pas_refined aag\<rbrace>"
-  apply (cases irq_ctl_inv; simp)
-  apply (wpsimp wp: cap_insert_pas_refined_not_transferable)
-   apply (clarsimp simp: cte_wp_at_caps_of_state clas_no_asid cap_links_irq_def
-                         authorised_irq_ctl_inv_def aag_cap_auth_def)
-  apply (wp arch_invoke_irq_control_pas_refined)
-  apply (clarsimp simp: cte_wp_at_caps_of_state clas_no_asid cap_links_irq_def
-                        authorised_irq_ctl_inv_def aag_cap_auth_def)
-  done
-
-definition
-  authorised_irq_hdl_inv :: "'a PAS \<Rightarrow> Invocations_A.irq_handler_invocation \<Rightarrow> bool"
-where
+definition authorised_irq_hdl_inv :: "'a PAS \<Rightarrow> Invocations_A.irq_handler_invocation \<Rightarrow> bool" where
   "authorised_irq_hdl_inv aag hinv \<equiv>
      case hinv of
          irq_handler_invocation.SetIRQHandler word cap x \<Rightarrow>
@@ -70,19 +23,64 @@ lemma emptyable_irq_node:
   by (simp add:emptyable_def tcb_cnode_index_def)
 
 lemma pas_refined_is_subject_irqD:
-  "\<lbrakk>is_subject_irq aag irq ; pas_refined aag s \<rbrakk> \<Longrightarrow> is_subject aag (interrupt_irq_node s irq)"
+  "\<lbrakk> is_subject_irq aag irq; pas_refined aag s \<rbrakk> \<Longrightarrow> is_subject aag (interrupt_irq_node s irq)"
   by (simp add:pas_refined_def irq_map_wellformed_aux_def)
 
+
+locale Interrupt_AC_1 =
+  fixes arch_authorised_irq_ctl_inv :: "'a PAS \<Rightarrow> arch_irq_control_invocation \<Rightarrow> bool"
+  assumes arch_invoke_irq_control_pas_refined:
+    "\<lbrace>pas_refined (aag :: 'a PAS) and valid_mdb and arch_irq_control_inv_valid irq_ctl_inv
+                                  and K (arch_authorised_irq_ctl_inv aag irq_ctl_inv)\<rbrace>
+     arch_invoke_irq_control irq_ctl_inv
+     \<lbrace>\<lambda>_. pas_refined aag\<rbrace>"
+  and arch_invoke_irq_handler_pas_refined:
+    "\<lbrace>pas_refined aag and invs and (\<lambda>s. interrupt_states s x1 \<noteq> IRQInactive)\<rbrace>
+     arch_invoke_irq_handler (ACKIrq x1)
+     \<lbrace>\<lambda>_. pas_refined aag\<rbrace>"
+  and arch_invoke_irq_control_respects:
+    "\<lbrace>integrity aag X st and pas_refined aag and K (arch_authorised_irq_ctl_inv aag acinv)\<rbrace>
+     arch_invoke_irq_control acinv
+     \<lbrace>\<lambda>_. integrity aag X st\<rbrace>"
+  and arch_invoke_irq_handler_respects:
+    "\<lbrace>integrity aag X st and pas_refined aag and einvs\<rbrace>
+     arch_invoke_irq_handler (ACKIrq x1)
+     \<lbrace>\<lambda>_. integrity aag X st\<rbrace>"
+  and arch_check_irq_inv[wp]:
+    "arch_check_irq irq \<lbrace>\<lambda>s :: det_ext state. P s\<rbrace>"
+begin
+
+definition authorised_irq_ctl_inv :: "'a PAS \<Rightarrow> Invocations_A.irq_control_invocation \<Rightarrow> bool" where
+  "authorised_irq_ctl_inv aag cinv \<equiv>
+     case cinv of
+       IRQControl irq x1 x2 \<Rightarrow> is_subject aag (fst x1) \<and> is_subject aag (fst x2) \<and>
+                               (pasSubject aag, Control, pasIRQAbs aag irq) \<in> pasPolicy aag
+     | ArchIRQControl acinv \<Rightarrow> arch_authorised_irq_ctl_inv aag acinv"
+
+lemma invoke_irq_control_pas_refined:
+  "\<lbrace>pas_refined aag and valid_mdb and irq_control_inv_valid irq_ctl_inv
+                    and K (authorised_irq_ctl_inv aag irq_ctl_inv)\<rbrace>
+   invoke_irq_control irq_ctl_inv
+   \<lbrace>\<lambda>_. pas_refined aag\<rbrace>"
+  apply (cases irq_ctl_inv; simp)
+  apply (wpsimp wp: cap_insert_pas_refined_not_transferable)
+   apply (clarsimp simp: cte_wp_at_caps_of_state clas_no_asid cap_links_irq_def
+                         authorised_irq_ctl_inv_def aag_cap_auth_def)
+  apply (wp arch_invoke_irq_control_pas_refined)
+  apply (clarsimp simp: cte_wp_at_caps_of_state clas_no_asid cap_links_irq_def
+                        authorised_irq_ctl_inv_def aag_cap_auth_def)
+  done
+
 lemma invoke_irq_handler_pas_refined:
-  "\<lbrace>pas_refined aag and invs and irq_handler_inv_valid irq_inv
-       and K (authorised_irq_hdl_inv aag irq_inv)\<rbrace>
-     invoke_irq_handler irq_inv
-   \<lbrace>\<lambda>rv (s::det_ext state). pas_refined aag s\<rbrace>"
+  "\<lbrace>pas_refined (aag :: 'a PAS) and invs and irq_handler_inv_valid irq_inv
+                                and K (authorised_irq_hdl_inv aag irq_inv)\<rbrace>
+   invoke_irq_handler irq_inv
+   \<lbrace>\<lambda>_ s. pas_refined aag s\<rbrace>"
   apply (rule hoare_gen_asm)
   apply (cases irq_inv, simp_all add: authorised_irq_hdl_inv_def)
-    apply (wp cap_insert_pas_refined_not_transferable delete_one_caps_of_state
-          | strengthen invs_mdb aag_Control_owns_strg
-          | simp add: pas_refined_wellformed cte_wp_at_caps_of_state)+
+    apply (wp arch_invoke_irq_handler_pas_refined)
+   apply (wp cap_insert_pas_refined_not_transferable delete_one_caps_of_state
+          | strengthen invs_mdb | simp add: cte_wp_at_caps_of_state)+
     apply (rename_tac irq cap slot)
     apply (rule_tac Q =
             "\<lambda> irq_slot. K(irq_slot \<noteq> slot) and invs and emptyable irq_slot
@@ -92,18 +90,16 @@ lemma invoke_irq_handler_pas_refined:
      apply (force simp: cte_wp_at_caps_of_state)
     apply simp
     apply (wp get_irq_slot_different)
-
    apply (clarsimp simp: emptyable_irq_node cte_wp_at_caps_of_state)
    apply (fastforce simp: interrupt_derived_def is_cap_simps cap_master_cap_def split: cap.splits)
   apply (wp delete_one_caps_of_state | simp add: get_irq_slot_def)+
   apply (fastforce dest: pas_refined_is_subject_irqD)
   done
 
-
 lemma invoke_irq_control_respects:
   "\<lbrace>integrity aag X st and pas_refined aag and K (authorised_irq_ctl_inv aag irq_ctl_inv)\<rbrace>
-     invoke_irq_control irq_ctl_inv
-   \<lbrace>\<lambda>y. integrity aag X st\<rbrace>"
+   invoke_irq_control irq_ctl_inv
+   \<lbrace>\<lambda>_. integrity aag X st\<rbrace>"
   apply (rule hoare_gen_asm)
   apply (cases irq_ctl_inv)
   subgoal \<comment>\<open>generic case\<close>
@@ -111,63 +107,63 @@ lemma invoke_irq_control_respects:
     apply (wp cap_insert_integrity_autarch aag_Control_into_owns_irq | simp | blast)+
     done
   subgoal for arch_irq_ctl_inv \<comment>\<open>arch case\<close>
-    apply (simp add: arch_authorised_irq_ctl_inv_def authorised_irq_ctl_inv_def)
-    apply (case_tac arch_irq_ctl_inv, clarsimp simp add: setIRQTrigger_def)
-    apply (wp cap_insert_integrity_autarch aag_Control_into_owns_irq dmo_mol_respects do_machine_op_pas_refined | simp)+
-    apply auto
+    apply (wpsimp wp: arch_invoke_irq_control_respects simp: authorised_irq_ctl_inv_def)
     done
   done
 
-lemma integrity_irq_masks [iff]:
-  "integrity aag X st (s\<lparr>machine_state := machine_state s \<lparr>irq_masks := v \<rparr>\<rparr>) = integrity aag X st s"
-  unfolding integrity_def
-  by simp
-
 lemma invoke_irq_handler_respects:
-  "\<lbrace>integrity aag X st and pas_refined aag and einvs and
-       K (authorised_irq_hdl_inv aag irq_inv)\<rbrace>
-     invoke_irq_handler irq_inv
-   \<lbrace>\<lambda>y. integrity aag X st\<rbrace>"
-  apply (rule hoare_gen_asm)
+  "\<lbrace>integrity (aag :: 'a PAS) X st and pas_refined aag and einvs
+                                   and K (authorised_irq_hdl_inv aag irq_inv)\<rbrace>
+   invoke_irq_handler irq_inv
+   \<lbrace>\<lambda>_. integrity aag X st\<rbrace>"
   apply (cases irq_inv, simp_all add: authorised_irq_hdl_inv_def)
+  by (wpsimp wp: arch_invoke_irq_handler_respects cap_insert_integrity_autarch)+
+
+end
+
+
+lemma decode_irq_handler_invocation_authorised [wp]:
+  "\<lbrace>K (is_subject_irq aag irq \<and> (\<forall>cap_slot \<in> set caps. pas_cap_cur_auth aag (fst cap_slot)
+                              \<and> is_subject aag (fst (snd cap_slot))))\<rbrace>
+   decode_irq_handler_invocation info_label irq caps
+   \<lbrace>\<lambda>x s. authorised_irq_hdl_inv aag x\<rbrace>, -"
+  unfolding decode_irq_handler_invocation_def authorised_irq_hdl_inv_def
   apply (rule hoare_pre)
-  apply (wp cap_insert_integrity_autarch get_irq_slot_owns dmo_wp | simp add: maskInterrupt_def )+
+   apply (simp add: Let_def split_def split del: if_split cong: if_cong)
+   apply wp
+  apply (auto dest!: hd_in_set)
   done
 
+
+locale Interrupt_AC_2 = Interrupt_AC_1 +
+  assumes arch_decode_irq_control_invocation_authorised:
+    "\<lbrace>pas_refined aag and
+      K (is_subject aag (fst slot) \<and> (\<forall>cap \<in> set caps. pas_cap_cur_auth aag cap) \<and>
+         (args \<noteq> [] \<longrightarrow> (pasSubject aag, Control, pasIRQAbs aag (ucast (args ! 0))) \<in> pasPolicy aag))\<rbrace>
+     arch_decode_irq_control_invocation info_label args slot caps
+     \<lbrace>\<lambda>x s. arch_authorised_irq_ctl_inv aag x\<rbrace>, -"
+begin
+
 lemma decode_irq_control_invocation_authorised [wp]:
-  "\<lbrace>pas_refined aag
-      and K (is_subject aag (fst slot)
-              \<and> (\<forall>cap \<in> set caps. pas_cap_cur_auth aag cap)
-              \<and> (args \<noteq> [] \<longrightarrow>
-                  (pasSubject aag, Control, pasIRQAbs aag (ucast (args ! 0))) \<in> pasPolicy aag))\<rbrace>
-    decode_irq_control_invocation info_label args slot caps
-  \<lbrace>\<lambda>x s. authorised_irq_ctl_inv aag x\<rbrace>, -"
-  unfolding decode_irq_control_invocation_def arch_decode_irq_control_invocation_def authorised_irq_ctl_inv_def arch_authorised_irq_ctl_inv_def arch_check_irq_def
+  "\<lbrace>pas_refined aag and
+    K (is_subject aag (fst slot) \<and> (\<forall>cap \<in> set caps. pas_cap_cur_auth aag cap) \<and>
+       (args \<noteq> [] \<longrightarrow> (pasSubject aag, Control, pasIRQAbs aag (ucast (args ! 0))) \<in> pasPolicy aag))\<rbrace>
+   decode_irq_control_invocation info_label args slot caps
+   \<lbrace>\<lambda>x s. authorised_irq_ctl_inv aag x\<rbrace>, -"
+  unfolding decode_irq_control_invocation_def authorised_irq_ctl_inv_def
   apply (rule hoare_gen_asmE)
   apply (rule hoare_pre)
    apply (simp add: Let_def split del: if_split cong: if_cong)
-   apply (wp whenE_throwError_wp hoare_vcg_imp_lift hoare_drop_imps
-         | strengthen  aag_Control_owns_strg
-         | simp add: o_def del: hoare_True_E_R)+
+   apply (wp arch_decode_irq_control_invocation_authorised
+             whenE_throwError_wp hoare_vcg_imp_lift hoare_drop_imps
+          | strengthen  aag_Control_owns_strg
+          | simp add: o_def del: hoare_True_E_R)+
   apply (cases args, simp_all)
   apply (cases caps, simp_all)
   apply (simp add: ucast_mask_drop)
   apply (auto simp: is_cap_simps cap_auth_conferred_def
                     pas_refined_wellformed
                     pas_refined_all_auth_is_owns aag_cap_auth_def)
-  done
-
-lemma decode_irq_handler_invocation_authorised [wp]:
-  "\<lbrace>K (is_subject_irq aag irq
-         \<and> (\<forall>cap_slot \<in> set caps. pas_cap_cur_auth aag (fst cap_slot)
-                                \<and> is_subject aag (fst (snd cap_slot))))\<rbrace>
-    decode_irq_handler_invocation info_label irq caps
-  \<lbrace>\<lambda>x s. authorised_irq_hdl_inv aag x\<rbrace>, -"
-  unfolding decode_irq_handler_invocation_def authorised_irq_hdl_inv_def
-  apply (rule hoare_pre)
-   apply (simp add: Let_def split_def split del: if_split cong: if_cong)
-   apply wp
-  apply (auto dest!: hd_in_set)
   done
 
 end
